json: Move away from member functions to reduce the number of lambdas
https://github.com/dafny-lang/dafny/issues/2179

src/JSON/JSON.Deserializer.dfy
@@ -1,6 +1,4 @@
-include "../BoundedInts.dfy"
-include "../Wrappers.dfy"
-include "Grammar.dfy"
+include "JSON.Grammar.dfy"
 include "Parsers.dfy"
 
 module {:options "-functionSyntax:4"} JSON.Deserializer {
@@ -13,10 +11,10 @@ module {:options "-functionSyntax:4"} JSON.Deserializer {
     import opened Grammar
 
     datatype JSONError =
-      | LeadingSeparator // "Separator not allowed before first item"
-      | UnterminatedSequence // "Unterminated sequence."
-      | EmptyNumber // "Number must contain at least one digit"
-      | ExpectingEOF // "Expecting EOF"
+      | LeadingSeparator
+      | UnterminatedSequence
+      | EmptyNumber
+      | ExpectingEOF
     {
       function ToString() : string {
         match this
@@ -33,24 +31,27 @@ module {:options "-functionSyntax:4"} JSON.Deserializer {
 
     // FIXME make more things opaque
 
-    function {:opaque} Get(ps: FreshCursor, err: JSONError): (pp: ParseResult<jchar>)
-      ensures pp.Success? ==> pp.value.t.Length() == 1
-      ensures pp.Success? ==> pp.value.ps.StrictlySplitFrom?(ps) // FIXME splitfrom should be on pp
+    function {:opaque} Get(ps: FreshCursor, err: JSONError): (pr: ParseResult<jchar>)
+      ensures pr.Success? ==> pr.value.t.Length() == 1
+      ensures pr.Success? ==> ps.Bytes() == pr.value.t.Bytes() + pr.value.ps.Bytes()
+      ensures pr.Success? ==> pr.value.ps.StrictlySplitFrom?(ps) // FIXME splitfrom should be on pp
     {
       var ps :- ps.Get(err);
       Success(ps.Split())
     }
 
     function {:opaque} WS(ps: FreshCursor): (pp: Split<jblanks>)
+      ensures ps.Bytes() == pp.t.Bytes() + pp.ps.Bytes()
       ensures pp.ps.SplitFrom?(ps)
     {
       ps.SkipWhile(Blank?).Split()
     }
 
     function Structural<T>(ps: FreshCursor, parser: Parser<T>)
-      : (ppr: ParseResult<Structural<T>>)
+      : (pr: ParseResult<Structural<T>>)
       requires forall ps :: parser.fn.requires(ps)
-      ensures ppr.Success? ==> ppr.value.ps.StrictlySplitFrom?(ps)
+      // PROOF: pass spec in here ensures pr.Success? ==> ps.Bytes() == pr.value.t.Bytes() + pr.value.ps.Bytes()
+      ensures pr.Success? ==> pr.value.ps.StrictlySplitFrom?(ps)
     {
       var SP(before, ps) := WS(ps);
       var SP(val, ps) :- parser.fn(ps);
@@ -70,12 +71,13 @@ module {:options "-functionSyntax:4"} JSON.Deserializer {
     const CLOSE: byte
     const SEPARATOR: byte
 
-    type TItem
-    function Item(ps: FreshCursor, json: SubParser<Value>)
-      : (ppr: ParseResult<TItem>)
+    type TElement // LATER: With traits, make sure that TElement is convertible to bytes
+    function Element(ps: FreshCursor, json: SubParser<Value>)
+      : (pr: ParseResult<TElement>)
       requires ps.StrictlySplitFrom?(json.ps)
       decreases ps.Length()
-      ensures ppr.Success? ==> ppr.value.ps.SplitFrom?(ps)
+      // PROOF pass spec here
+      ensures pr.Success? ==> pr.value.ps.SplitFrom?(ps)
   }
 
   abstract module Sequences {
@@ -92,17 +94,18 @@ module {:options "-functionSyntax:4"} JSON.Deserializer {
     type jopen = v: View | v.Byte?(OPEN) witness View.OfBytes([OPEN])
     type jclose = v: View | v.Byte?(CLOSE) witness View.OfBytes([CLOSE])
     type jsep = v: View | v.Byte?(SEPARATOR) witness View.OfBytes([SEPARATOR])
-    type TSeq = Bracketed<jopen, jsep, TItem, jclose>
+    type TSeq = Bracketed<jopen, jsep, TElement, jclose>
 
-    function {:tailrecursion} SeparatorPrefixedItems(
+    function {:tailrecursion} SeparatorPrefixedElements(
       ps: FreshCursor, json: SubParser<Value>,
       open: Structural<jopen>,
-      items: PrefixedSequence<jsep, TItem>
-    ): (ppr: ParseResult<TSeq>)
+      items: PrefixedSequence<jsep, TElement>
+    ): (pr: ParseResult<TSeq>)
       requires ps.StrictlySplitFrom?(json.ps)
       requires NoLeadingPrefix(items)
       decreases ps.Length()
-      ensures ppr.Success? ==> ppr.value.ps.StrictlySplitFrom?(ps)
+      // PROOF ensures pr.Success? ==> ps.Bytes() == pr.value.t.Bytes() + pr.value.ps.Bytes()
+      ensures pr.Success? ==> pr.value.ps.StrictlySplitFrom?(ps)
     {
       var SP(sep, ps) :- Core.Structural(ps, Parsers.Parser(ps => Get(ps, UnterminatedSequence)));
       var s0 := sep.t.At(0);
@@ -110,43 +113,43 @@ module {:options "-functionSyntax:4"} JSON.Deserializer {
         Success(SP(Grammar.Bracketed(open, items, sep), ps))
       else if s0 == SEPARATOR then
         :- Need(|items| > 0, OtherError(LeadingSeparator));
-        var SP(item, ps) :- Item(ps, json);
+        var SP(item, ps) :- Element(ps, json);
         var items := items + [Prefixed(NonEmpty(sep), item)];
-        ghost var ppr' := SeparatorPrefixedItems(ps, json, open, items); // DISCUSS: Why is this needed?
-        assert ppr'.Success? ==> ppr'.value.ps.StrictlySplitFrom?(ps);
-        SeparatorPrefixedItems(ps, json, open, items)
+        ghost var pr' := SeparatorPrefixedElements(ps, json, open, items); // DISCUSS: Why is this needed?
+        assert pr'.Success? ==> pr'.value.ps.StrictlySplitFrom?(ps);
+        SeparatorPrefixedElements(ps, json, open, items)
       else
         Failure(ExpectingAnyByte([CLOSE, SEPARATOR], s0 as opt_byte))
     }
 
     function Open(ps: FreshCursor)
-      : (ppr: ParseResult<jopen>)
+      : (pr: ParseResult<jopen>)
     {
       var ps :- ps.AssertByte(OPEN);
       Success(ps.Split())
     }
 
     function Close(ps: FreshCursor)
-      : (ppr: ParseResult<jclose>)
+      : (pr: ParseResult<jclose>)
     {
       var ps :- ps.AssertByte(CLOSE);
       Success(ps.Split())
     }
 
-    function Items(ps: FreshCursor, json: SubParser<Value>, open: Structural<jopen>)
-      : (ppr: ParseResult<TSeq>)
+    function Elements(ps: FreshCursor, json: SubParser<Value>, open: Structural<jopen>)
+      : (pr: ParseResult<TSeq>)
       requires ps.StrictlySplitFrom?(json.ps)
-      ensures ppr.Success? ==> ppr.value.ps.StrictlySplitFrom?(ps)
+      ensures pr.Success? ==> pr.value.ps.StrictlySplitFrom?(ps)
     {
       if ps.Peek() == CLOSE as opt_byte then
         var SP(close, ps) :- Core.Structural(ps, Parsers.Parser(Close));
         Success(SP(Grammar.Bracketed(open, [], close), ps))
       else
-        var SP(item, ps) :- Item(ps, json);
+        var SP(item, ps) :- Element(ps, json);
         var items := [Prefixed(Empty(), item)];
-        ghost var ppr' := SeparatorPrefixedItems(ps, json, open, items); // DISCUSS: Why is this needed?
-        assert ppr'.Success? ==> ppr'.value.ps.StrictlySplitFrom?(ps);
-        SeparatorPrefixedItems(ps, json, open, items)
+        ghost var pr' := SeparatorPrefixedElements(ps, json, open, items); // DISCUSS: Why is this needed?
+        assert pr'.Success? ==> pr'.value.ps.StrictlySplitFrom?(ps);
+        SeparatorPrefixedElements(ps, json, open, items)
     }
 
     lemma Valid(x: TSeq)
@@ -154,29 +157,29 @@ module {:options "-functionSyntax:4"} JSON.Deserializer {
       ensures x.r.t.Byte?(CLOSE)
       ensures NoLeadingPrefix(x.data)
       ensures forall pf | pf in x.data ::
-        pf.before.NonEmpty? ==> pf.before.t.t.Byte?(SEPARATOR)
+        pf.prefix.NonEmpty? ==> pf.prefix.t.t.Byte?(SEPARATOR)
     { // DISCUSS: Why is this lemma needed?  Why does it require a body?
       var xlt: jopen := x.l.t;
       var xrt: jclose := x.r.t;
       forall pf | pf in x.data
-        ensures pf.before.NonEmpty? ==> pf.before.t.t.Byte?(SEPARATOR)
+        ensures pf.prefix.NonEmpty? ==> pf.prefix.t.t.Byte?(SEPARATOR)
       {
-        if pf.before.NonEmpty? {
-          var xtt := pf.before.t.t;
+        if pf.prefix.NonEmpty? {
+          var xtt := pf.prefix.t.t;
         }
       }
     }
 
     function Bracketed(ps: FreshCursor, json: SubParser<Value>)
-      : (ppr: ParseResult<TSeq>)
+      : (pr: ParseResult<TSeq>)
       requires ps.SplitFrom?(json.ps)
-      ensures ppr.Success? ==> ppr.value.ps.StrictlySplitFrom?(ps)
-      // ensures ppr.Success? ==> Valid?(ppr.value.t)
+      ensures pr.Success? ==> pr.value.ps.StrictlySplitFrom?(ps)
+      // ensures pr.Success? ==> Valid?(pr.value.t)
     {
       var SP(open, ps) :- Core.Structural(ps, Parsers.Parser(Open));
-      ghost var ppr := Items(ps, json, open); // DISCUSS: Why is this needed?
-      assert ppr.Success? ==> ppr.value.ps.StrictlySplitFrom?(ps);
-      Items(ps, json, open)
+      ghost var pr := Elements(ps, json, open); // DISCUSS: Why is this needed?
+      assert pr.Success? ==> pr.value.ps.StrictlySplitFrom?(ps);
+      Elements(ps, json, open)
     }
   }
 
@@ -189,8 +192,8 @@ module {:options "-functionSyntax:4"} JSON.Deserializer {
     import opened Core
     import Values
 
-    function JSON(ps: FreshCursor) : (ppr: ParseResult<JSON>)
-      ensures ppr.Success? ==> ppr.value.ps.StrictlySplitFrom?(ps)
+    function JSON(ps: FreshCursor) : (pr: ParseResult<JSON>)
+      ensures pr.Success? ==> pr.value.ps.StrictlySplitFrom?(ps)
     {
       Core.Structural(ps, Parsers.Parser(Values.Value))
     }
@@ -216,9 +219,9 @@ module {:options "-functionSyntax:4"} JSON.Deserializer {
     import Arrays
     import Constants
 
-    function Value(ps: FreshCursor) : (ppr: ParseResult<Value>)
+    function Value(ps: FreshCursor) : (pr: ParseResult<Value>)
       decreases ps.Length(), 1
-      ensures ppr.Success? ==> ppr.value.ps.StrictlySplitFrom?(ps)
+      ensures pr.Success? ==> pr.value.ps.StrictlySplitFrom?(ps)
     {
       var c := ps.Peek();
       if c == '{' as opt_byte then
@@ -263,9 +266,9 @@ module {:options "-functionSyntax:4"} JSON.Deserializer {
     import opened Core
     import opened Cursors
 
-    function Constant(ps: FreshCursor, expected: bytes) : (ppr: ParseResult<jstring>)
+    function Constant(ps: FreshCursor, expected: bytes) : (pr: ParseResult<jstring>)
       requires |expected| < TWO_TO_THE_32
-      ensures ppr.Success? ==> ppr.value.t.Bytes() == expected
+      ensures pr.Success? ==> pr.value.t.Bytes() == expected
     {
       var ps :- ps.AssertBytes(expected);
       Success(ps.Split())
@@ -282,8 +285,8 @@ module {:options "-functionSyntax:4"} JSON.Deserializer {
     import opened Parsers
     import opened Core
 
-    function String(ps: FreshCursor): (ppr: ParseResult<jstring>)
-      ensures ppr.Success? ==> ppr.value.ps.StrictlySplitFrom?(ps)
+    function String(ps: FreshCursor): (pr: ParseResult<jstring>)
+      ensures pr.Success? ==> pr.value.ps.StrictlySplitFrom?(ps)
     {
       var ps :- ps.AssertChar('\"');
       var ps :- ps.SkipWhileLexer(StringBody, Partial(StringBodyLexerStart));
@@ -307,8 +310,8 @@ module {:options "-functionSyntax:4"} JSON.Deserializer {
       ps.SkipWhile(Digit?).Split()
     }
 
-    function NonEmptyDigits(ps: FreshCursor) : (ppr: ParseResult<jnum>)
-      ensures ppr.Success? ==> ppr.value.ps.StrictlySplitFrom?(ps)
+    function NonEmptyDigits(ps: FreshCursor) : (pr: ParseResult<jnum>)
+      ensures pr.Success? ==> pr.value.ps.StrictlySplitFrom?(ps)
     {
       var pp := Digits(ps);
       :- Need(!pp.t.Empty?, OtherError(EmptyNumber));
@@ -327,16 +330,16 @@ module {:options "-functionSyntax:4"} JSON.Deserializer {
       ps.SkipIf(c => c == '-' as byte || c == '+' as byte).Split()
     }
 
-    function TrimmedInt(ps: FreshCursor) : (ppr: ParseResult<jint>)
-      ensures ppr.Success? ==> ppr.value.ps.StrictlySplitFrom?(ps)
+    function TrimmedInt(ps: FreshCursor) : (pr: ParseResult<jint>)
+      ensures pr.Success? ==> pr.value.ps.StrictlySplitFrom?(ps)
     {
       var pp := ps.SkipIf(c => c == '0' as byte).Split();
       if pp.t.Empty? then NonEmptyDigits(ps)
       else Success(pp)
     }
 
-    function Exp(ps: FreshCursor) : (ppr: ParseResult<Maybe<jexp>>)
-      ensures ppr.Success? ==> ppr.value.ps.SplitFrom?(ps)
+    function Exp(ps: FreshCursor) : (pr: ParseResult<Maybe<jexp>>)
+      ensures pr.Success? ==> pr.value.ps.SplitFrom?(ps)
     {
       var SP(e, ps) :=
         ps.SkipIf(c => c == 'e' as byte || c == 'E' as byte).Split();
@@ -349,8 +352,8 @@ module {:options "-functionSyntax:4"} JSON.Deserializer {
         Success(SP(NonEmpty(JExp(e, sign, num)), ps))
     }
 
-    function Frac(ps: FreshCursor) : (ppr: ParseResult<Maybe<jfrac>>)
-      ensures ppr.Success? ==> ppr.value.ps.SplitFrom?(ps)
+    function Frac(ps: FreshCursor) : (pr: ParseResult<Maybe<jfrac>>)
+      ensures pr.Success? ==> pr.value.ps.SplitFrom?(ps)
     {
       var SP(period, ps) :=
         ps.SkipIf(c => c == '.' as byte).Split();
@@ -361,9 +364,9 @@ module {:options "-functionSyntax:4"} JSON.Deserializer {
         Success(SP(NonEmpty(JFrac(period, num)), ps))
     }
 
-    function Number(ps: FreshCursor) : (ppr: ParseResult<Value>)
-      ensures ppr.Success? ==> ppr.value.ps.StrictlySplitFrom?(ps)
-      ensures ppr.Success? ==> ppr.value.t.Number?
+    function Number(ps: FreshCursor) : (pr: ParseResult<Value>)
+      ensures pr.Success? ==> pr.value.ps.StrictlySplitFrom?(ps)
+      ensures pr.Success? ==> pr.value.t.Number?
     {
       var SP(minus, ps) := Minus(ps);
       var SP(num, ps) :- TrimmedInt(ps);
@@ -377,14 +380,14 @@ module {:options "-functionSyntax:4"} JSON.Deserializer {
     import opened Strings
     import opened Wrappers
 
-    type TItem = Value
+    type TElement = Value
 
     const OPEN := '[' as byte
     const CLOSE := ']' as byte
     const SEPARATOR: byte := ',' as byte
 
-    function Item(ps: FreshCursor, json: SubParser<Value>)
-      : (ppr: ParseResult<TItem>)
+    function Element(ps: FreshCursor, json: SubParser<Value>)
+      : (pr: ParseResult<TElement>)
     {
       assert ps.StrictlySplitFrom?(json.ps);
       assert json.Valid?();
@@ -402,21 +405,21 @@ module {:options "-functionSyntax:4"} JSON.Deserializer {
     import opened Wrappers
     import Strings
 
-    type TItem = jkv
+    type TElement = jkv
 
     const OPEN := '{' as byte
     const CLOSE := '}' as byte
     const SEPARATOR: byte := ',' as byte
 
     function Colon(ps: FreshCursor)
-      : (ppr: ParseResult<jcolon>)
+      : (pr: ParseResult<jcolon>)
     {
       var ps :- ps.AssertChar(':');
       Success(ps.Split())
     }
 
-    function Item(ps: FreshCursor, json: SubParser<Value>)
-      : (ppr: ParseResult<TItem>)
+    function Element(ps: FreshCursor, json: SubParser<Value>)
+      : (pr: ParseResult<TElement>)
     {
       var SP(k, ps) :- Strings.String(ps);
       var SP(colon, ps) :- Core.Structural(ps, Parsers.Parser(Colon));
