src/JSON/JSON.Grammar.dfy
@@ -1,0 +1,78 @@
+include "../BoundedInts.dfy"
+include "Views.dfy"
+
+module {:options "-functionSyntax:4"} JSON.Grammar {
+  import opened BoundedInts
+  import opened Views.Core
+
+  type jchar = v: View | v.Length() == 1 witness View.OfBytes(['b' as byte])
+  type jperiod = v: View | v.Char?('.') witness View.OfBytes(['.' as byte])
+  type je = v: View | v.Char?('e') || v.Char?('E') witness View.OfBytes(['e' as byte])
+  type jcolon = v: View | v.Char?(':') witness View.OfBytes([':' as byte])
+  type jcomma = v: View | v.Char?(',') witness View.OfBytes([',' as byte])
+  type jlbrace = v: View | v.Char?('{') witness View.OfBytes(['{' as byte])
+  type jrbrace = v: View | v.Char?('}') witness View.OfBytes(['}' as byte])
+  type jlbracket = v: View | v.Char?('[') witness View.OfBytes(['[' as byte])
+  type jrbracket = v: View | v.Char?(']') witness View.OfBytes([']' as byte])
+  type jminus = v: View | v.Char?('-') || v.Empty? witness View.OfBytes([])
+  type jsign = v: View | v.Char?('-') || v.Char?('+') || v.Empty? witness View.OfBytes([])
+
+  predicate Blank?(b: byte) { b == 0x20 || b == 0x09 || b == 0x0A || b == 0x0D }
+  ghost predicate Blanks?(v: View) { forall b | b in v.Bytes() :: Blank?(b) }
+  type jblanks = v: View | Blanks?(v) witness View.OfBytes([])
+
+  datatype Structural<+T> =
+    Structural(before: jblanks, t: T, after: jblanks)
+
+  datatype Maybe<+T> = Empty() | NonEmpty(t: T)
+
+  datatype Prefixed<+S, +T> =
+    Prefixed(prefix: Maybe<Structural<S>>, t: T)
+
+  type PrefixedSequence<+S, +D> = s: seq<Prefixed<S, D>> | NoLeadingPrefix(s)
+  ghost predicate NoLeadingPrefix<S, D>(s: seq<Prefixed<S, D>>) {
+    forall idx | 0 <= idx < |s| :: s[idx].prefix.Empty? <==> idx == 0
+  }
+
+  datatype Bracketed<+L, +S, +D, +R> =
+    Bracketed(l: Structural<L>, data: PrefixedSequence<S, D>, r: Structural<R>)
+
+  const NULL: bytes := ['n' as byte, 'u' as byte, 'l' as byte, 'l' as byte]
+  const TRUE: bytes := ['t' as byte, 'r' as byte, 'u' as byte, 'e' as byte]
+  const FALSE: bytes := ['f' as byte, 'a' as byte, 'l' as byte, 's' as byte, 'e' as byte]
+
+  ghost predicate Null?(v: View) { v.Bytes() == NULL }
+  ghost predicate Bool?(v: View) { v.Bytes() in {TRUE, FALSE} }
+  predicate Digit?(b: byte) { '0' as byte <= b <= '9' as byte }
+  ghost predicate Digits?(v: View) { forall b | b in v.Bytes() :: Digit?(b) }
+  ghost predicate Num?(v: View) { Digits?(v) && !v.Empty? }
+  ghost predicate Int?(v: View) { v.Char?('0') || (Num?(v) && v.At(0) != '0' as byte) }
+
+  type jstring = v: View | true witness View.OfBytes([]) // TODO: Enforce correct escaping
+  type jnull = v: View | Null?(v) witness View.OfBytes(NULL)
+  type jbool = v: View | Bool?(v) witness View.OfBytes(TRUE)
+  type jdigits = v: View | Digits?(v) witness View.OfBytes([])
+  type jnum = v: View | Num?(v) witness View.OfBytes(['0' as byte])
+  type jint = v: View | Int?(v) witness View.OfBytes(['0' as byte])
+  datatype jkv = KV(k: jstring, colon: Structural<jcolon>, v: Value)
+
+  type jobject = Bracketed<jlbrace, jcomma, jkv, jrbrace>
+  type jarray = Bracketed<jlbracket, jcomma, Value, jrbracket>
+  type jmembers = PrefixedSequence<jcomma, jkv>
+  type jmember = Prefixed<jcomma, jkv>
+  type jitems = PrefixedSequence<jcomma, Value>
+  type jitem = Prefixed<jcomma, Value>
+
+  datatype jfrac = JFrac(period: jperiod, num: jnum)
+  datatype jexp = JExp(e: je, sign: jsign, num: jnum)
+
+  datatype Value =
+    | Null(n: jnull)
+    | Bool(b: jbool)
+    | String(str: jstring)
+    | Number(minus: jminus, num: jnum, frac: Maybe<jfrac>, exp: Maybe<jexp>)
+    | Object(obj: jobject)
+    | Array(arr: jarray)
+
+  type JSON = Structural<Value>
+}
