src/JSON/JSON.Spec.dfy
@@ -1,0 +1,85 @@
+include "JSON.Grammar.dfy"
+
+module {:options "-functionSyntax:4"} JSON.Spec {
+  import opened BoundedInts
+
+  import Vs = Views.Core
+  import opened Grammar
+
+  function View(v: Vs.View) : bytes {
+    v.Bytes()
+  }
+
+  function Structural<T>(self: Structural<T>, pt: T -> bytes): bytes {
+    View(self.before) + pt(self.t) + View(self.after)
+  }
+
+  function StructuralView(self: Structural<Vs.View>): bytes {
+    Structural<Vs.View>(self, View)
+  }
+
+  function Maybe<T>(self: Maybe<T>, pt: T -> bytes): (bs: bytes)
+    ensures self.Empty? ==> bs == []
+    ensures self.NonEmpty? ==> bs == pt(self.t)
+  {
+    if self.Empty? then [] else pt(self.t)
+  }
+
+  function ConcatBytes<T>(ts: seq<T>, pt: T --> bytes) : bytes
+    requires forall d | d in ts :: pt.requires(d)
+  {
+    if |ts| == 0 then []
+    else pt(ts[0]) + ConcatBytes(ts[1..], pt)
+  }
+
+  function Bracketed<S, D>(self: Bracketed<Vs.View, S, D, Vs.View>, pdatum: Prefixed<S, D> --> bytes): bytes
+    requires forall d | d in self.data :: pdatum.requires(d)
+  {
+    StructuralView(self.l) +
+    ConcatBytes(self.data, pdatum) +
+    StructuralView(self.r)
+  }
+
+  function KV(self: jkv): bytes {
+    View(self.k) + StructuralView(self.colon) + Value(self.v)
+  }
+
+  function Frac(self: jfrac): bytes {
+    View(self.period) + View(self.num)
+  }
+
+  function Exp(self: jexp): bytes {
+    View(self.e) + View(self.sign) + View(self.num)
+  }
+
+  function Member(self: jmember) : bytes {
+    // BUG(https://github.com/dafny-lang/dafny/issues/2179)
+    Maybe<Structural<Vs.View>>(self.prefix, StructuralView) + KV(self.t)
+  }
+
+  function Item(self: jitem) : bytes {
+    // BUG(https://github.com/dafny-lang/dafny/issues/2179)
+    Maybe<Structural<Vs.View>>(self.prefix, StructuralView) + Value(self.t)
+  }
+
+  function Value(self: Value): bytes {
+    match self {
+      case Null(n) =>
+        View(n)
+      case Bool(b) =>
+        View(b)
+      case String(str) =>
+        View(str)
+      case Number(minus, num, frac, exp) =>
+        View(minus) + View(num) + Maybe(frac, Frac) + Maybe(exp, Exp)
+      case Object(obj) =>
+        Bracketed(obj, (d: jmember) requires d in obj.data => Member(d))
+      case Array(arr) =>
+        Bracketed(arr, (d: jitem) requires d in arr.data => Item(d))
+    }
+  }
+
+  function JSON(js: JSON) : bytes {
+    Structural(js, Value)
+  }
+}
